WIP hoare simulation

examples/multwhile/MultWhile01proof.v
@@ -53,24 +53,102 @@ Section SIMMODSEM.
   Context `{Σ: GRA.t}.
 
   (* trivial invariant *)
-  Let wf := mk_wf (fun (_: unit) _ _ => (True: iProp)%I).
+  Let Inv := (fun (_: unit) (_ _: Any.t) => (True: iProp)%I).
+
+  Definition to_irel (R_src R_tgt: Type)
+             (RR: R_src -> R_tgt -> Any.t -> Any.t -> iProp)
+             (st_src: Any.t) (st_tgt: Any.t)
+             (r_src: R_src) (r_tgt: R_tgt): Prop :=
+    exists mr_src mp_src,
+      (<<SRC: st_src = Any.pair mp_src (Any.upcast mr_src)>>) /\
+      (<<IPROP: RR r_src r_tgt mp_src st_tgt mr_src>>).
+
+  Lemma hbind_clo
+        A (a: shelve__ A)
+        mn r rg n m mr_src mp_src a0
+        X (Q: option mname -> X -> Any.t -> Any.t -> Σ -> Prop)
+        x vret_src vret_tgt
+        mp_tgt
+        (le: A -> A -> Prop)
+        (eqr: Any.t -> Any.t -> Any.t -> Any.t -> Prop)
+        (R: A -> Any.t -> Any.t -> iProp)
+        (R_src0 R_tgt0 R_src1 R_tgt1: Type)
+        (RR: R_src0 -> R_tgt0 -> Any.t -> Any.t -> iProp)
+
+        (itr_src: itree Es (Σ * R_src0)) (ktr_src: (Σ * R_src0) -> itree Es R_src1)
+        (itr_tgt: itree Es R_tgt) (ktr_tgt: R_tgt0 -> itree Es R_tgt1)
+
+        ctx l
+        (ACC: current_iPropL ctx l)
+
+        (WLE: le a0 a)
+
+        (UPDATABLE:
+           (from_iPropL l) ⊢ #=> (R a mp_src mp_tgt ** (Q mn x vret_src vret_tgt: iProp)))
+
+        (LEFT: gpaco8 (_sim_itree (mk_wf R) le) (cpn8 (_sim_itree (mk_wf R) le))
+                      r rg _ _ (to_irel RR) m n a0
+                      (Any.pair mp_src mr_src, itr_src)
+                      (mp_tgt, itr_tgt))
+        (LEFT: forall mr_src mp_src mp_tgt r_src r_tgt
+                      (RR: RR mp_src mp_tgt r_src r_tgt
+
+gpaco8 (_sim_itree (mk_wf R) le) (cpn8 (_sim_itree (mk_wf R) le))
+                      r rg _ _ RR m n a0
+                      (Any.pair mp_src mr_src, itr_src)
+                      (mp_tgt, itr_tgt))
+
+
+        (EQ: forall (mr_src1: Σ) (WLE: le a0 a) (WF: mk_wf R a (Any.pair mp_src mr_src1↑, mp_tgt)),
+            eqr (Any.pair mp_src mr_src1↑) mp_tgt vret_tgt vret_tgt)
+    :
+      gpaco8 (_sim_itree (mk_wf R) le) (cpn8 (_sim_itree (mk_wf R) le))
+             r rg _ _ eqr m n a0
+             (Any.pair mp_src mr_src, itr_src >>= ktr_src)
+             (mp_tgt, itr_tgt >>= ktr_tgt)
+  .
+  Proof.
+    subst. unfold HoareFunRet, mput, mget, guarantee.
+    repeat (ired_both; apply sim_itreeC_spec; econs). exists vret_tgt.
+    repeat (ired_both; apply sim_itreeC_spec; econs).
+    assert (exists mr_src1 rret_src,
+               (<<UPDATABLE: URA.wf (ctx ⋅ (mr_src1 ⋅ rret_src))>>) /\
+               (<<RSRC: R a mp_src mp_tgt mr_src1>>) /\
+               (<<PRE: Q mn x vret_src vret_tgt rret_src>>)).
+    { red in ACC. inv ACC. uipropall.
+      hexploit (UPDATABLE r0); et.
+      { eapply URA.wf_mon; et. }
+      i. des. subst. exists a1, b. splits; et.
+      replace (ctx ⋅ (a1 ⋅ b)) with (a1 ⋅ b ⋅ ctx); et.
+      r_solve.
+    }
+    des. exists (rret_src, mr_src1).
+    repeat (ired_both; apply sim_itreeC_spec; econs).
+    repeat (ired_both; apply sim_itreeC_spec; econs). unshelve esplits.
+    { r_wf UPDATABLE0. }
+    repeat (ired_both; apply sim_itreeC_spec; econs). unshelve esplits; eauto.
+    repeat (ired_both; apply sim_itreeC_spec; econs).
+    eapply EQ; et. econs; et.
+  Qed.
+
 
   Theorem correct: refines2 [MultWhile0.Mul] [MultWhile1.Mul].
   Proof.
     (* boring part *)
     eapply adequacy_local2. econs; ss.
-    i. econstructor 1 with (wf:=wf) (le:=top2); et.
+    i. econstructor 1 with (wf:=mk_wf Inv) (le:=top2); et.
     { ss. }
-    2: { exists tt. econs; ss; red; uipropall. }
+    2: { exists tt. unfold Inv. econs; ss; red; uipropall. }
     econs; ss. unfold mulF, ccallU. init. harg.
 
-    destruct x as [a b]. mDesAll. des; clarify. steps. astop. steps.
+    destruct x as [a b]. mDesAll. des; clarify. simpl. steps. astop. simpl. steps.
+    (* bind *)
     guclo lbindC_spec. eapply lbindR_intro with (RR := fun st_src _ r_src r_tgt => r_src = r_tgt↑ /\ r_tgt = (a * b)%Z /\ st_src = Any.pair mp_src (Any.upcast mr_src)).
-    { steps. deflag. instantiate (1:=tt).
+    { steps. instantiate (1:=tt).
       (* induction on a *)
       assert (exists n, <<EQ: a = Z.of_nat n>> /\ <<SUM: (a * b + 0 = a * b)%Z>>).
       { exists (Z.to_nat a). rewrite Z2Nat.id; auto. splits; auto. lia. }
-      des. revert EQ SUM. generalize a at 1 2 5. generalize 0%Z at 1 3. induction n; i.
+      des. deflag. revert EQ SUM. generalize a at 1 2 5. generalize 0%Z at 1 3. induction n; i.
       (* a = 0 *)
       { rewrite unfold_iter. subst. ss. steps. force_l. eexists. steps. }
       (* a = S _ *)
