proofmode/HSim.v
@@ -1,0 +1,1648 @@
+Require Import Coqlib.
+Require Import STS.
+Require Import Behavior.
+Require Import ModSem.
+Require Import Skeleton.
+Require Import PCM.
+Require Import Any.
+Require Import HoareDef OpenDef STB SimModSem.
+
+Require Import Relation_Definitions.
+Require Import Relation_Operators.
+Require Import RelationPairs.
+From ExtLib Require Import
+     Data.Map.FMapAList.
+Require Import Red IRed.
+Require Import ProofMode Invariant.
+Require Import HTactics.
+
+Set Implicit Arguments.
+
+Ltac ired_l := try (prw _red_gen 2 1 0).
+Ltac ired_r := try (prw _red_gen 1 1 0).
+
+Ltac ired_both := ired_l; ired_r.
+
+
+
+(* "safe" simulation constructors *)
+Section SIM.
+  Context `{Σ: GRA.t}.
+  Variable world: Type.
+  Variable le: relation world.
+  Variable I: world -> Any.t -> Any.t -> iProp.
+
+  Variable mn: mname.
+  Variable stb: gname -> option fspec.
+  Variable o: ord.
+
+  Inductive _hsim
+            (hsim: forall R_src R_tgt
+                          (Q: Any.t -> Any.t -> R_src -> R_tgt -> iProp)
+                          (ctx: Σ),
+                option ord -> bool -> bool -> Any.t * itree hEs R_src -> Any.t * itree Es R_tgt -> Prop)
+            {R_src R_tgt}
+            (Q: Any.t -> Any.t -> R_src -> R_tgt -> iProp)
+            (ctx: Σ)
+    : option ord -> bool -> bool -> Any.t * itree hEs R_src -> Any.t * itree Es R_tgt -> Prop :=
+  | hsim_ret
+      v_src v_tgt
+      st_src st_tgt
+      fuel f_src f_tgt
+      (RET: current_iProp ctx (Q st_src st_tgt v_src v_tgt))
+    :
+      _hsim hsim Q ctx fuel f_src f_tgt (st_src, (Ret v_src)) (st_tgt, (Ret v_tgt))
+  | hsim_call
+      fsp (x: fsp.(meta)) w0 FR
+      fn arg_src arg_tgt
+      st_src0 st_tgt0 ktr_src ktr_tgt
+      fuel f_src f_tgt
+      (SPEC: stb fn = Some fsp)
+      (PRE: current_iProp ctx (FR ** I w0 st_src0 st_tgt0 ** fsp.(precond) (Some mn) x arg_src arg_tgt))
+      (MEASURE: o = ord_top)
+      (POST: forall ctx1 w1 st_src1 st_tgt1 ret_src ret_tgt
+                    (ACC: current_iProp ctx1 (FR ** I w1 st_src1 st_tgt1 ** fsp.(postcond) (Some mn) x ret_src ret_tgt)),
+          hsim _ _ Q ctx1 None true true (st_src1, ktr_src ret_src) (st_tgt1, ktr_tgt ret_tgt))
+    :
+      _hsim hsim Q ctx fuel f_src f_tgt (st_src0, trigger (Call fn arg_src) >>= ktr_src) (st_tgt0, trigger (Call fn arg_tgt) >>= ktr_tgt)
+  | hsim_apc_start
+      fuel1
+      st_src st_tgt ktr_src itr_tgt
+      fuel f_src f_tgt
+      (SIM: _hsim hsim Q ctx (Some (ord_pure fuel1)) true f_tgt (st_src, ktr_src tt) (st_tgt, itr_tgt))
+    :
+      _hsim hsim Q ctx fuel f_src f_tgt (st_src, trigger (hAPC) >>= ktr_src) (st_tgt, itr_tgt)
+  | hsim_apc_step
+      fsp (x: fsp.(meta)) w0 FR arg_src
+      fn arg_tgt
+      st_src0 st_tgt0 itr_src ktr_tgt
+      fuel0 f_src f_tgt
+      (SPEC: stb fn = Some fsp)
+      (PRE: current_iProp ctx (FR ** I w0 st_src0 st_tgt0 ** fsp.(precond) (Some mn) x arg_src arg_tgt))
+      (MEASURE: ord_lt (fsp.(measure) x) o)
+      (POST: exists fuel1,
+          (<<FUEL: ord_lt fuel1 fuel0>>) /\
+          (<<SIM: forall ctx1 w1 st_src1 st_tgt1 ret_src ret_tgt
+                         (ACC: current_iProp ctx1 (FR ** I w1 st_src1 st_tgt1 ** fsp.(postcond) (Some mn) x ret_src ret_tgt)),
+              hsim _ _ Q ctx1 (Some fuel1) true true (st_src1, itr_src) (st_tgt1, ktr_tgt ret_tgt)>>))
+    :
+      _hsim hsim Q ctx (Some fuel0) f_src f_tgt (st_src0, itr_src) (st_tgt0, trigger (Call fn arg_tgt) >>= ktr_tgt)
+  | hsim_syscall
+      fn arg rvs
+      st_src st_tgt ktr_src ktr_tgt
+      fuel f_src f_tgt
+      (POST: forall ret,
+          hsim _ _ Q ctx None true true (st_src, ktr_src ret) (st_tgt, ktr_tgt ret))
+    :
+      _hsim hsim Q ctx fuel f_src f_tgt (st_src, trigger (Syscall fn arg rvs) >>= ktr_src) (st_tgt, trigger (Syscall fn arg rvs) >>= ktr_tgt)
+  | hsim_tau_src
+      st_src st_tgt itr_src itr_tgt
+      fuel f_src f_tgt
+      (SIM: _hsim hsim Q ctx None true f_tgt (st_src, itr_src) (st_tgt, itr_tgt))
+    :
+      _hsim hsim Q ctx fuel f_src f_tgt (st_src, tau;; itr_src) (st_tgt, itr_tgt)
+  | hsim_tau_tgt
+      st_src st_tgt itr_src itr_tgt
+      fuel f_src f_tgt
+      (SIM: _hsim hsim Q ctx fuel f_src true (st_src, itr_src) (st_tgt, itr_tgt))
+    :
+      _hsim hsim Q ctx fuel f_src f_tgt (st_src, itr_src) (st_tgt, tau;; itr_tgt)
+  | hsim_choose_src
+      X
+      st_src st_tgt ktr_src itr_tgt
+      fuel f_src f_tgt
+      (SIM: exists x, _hsim hsim Q ctx None true f_tgt (st_src, ktr_src x) (st_tgt, itr_tgt))
+    :
+      _hsim hsim Q ctx fuel f_src f_tgt (st_src, trigger (Choose X) >>= ktr_src) (st_tgt, itr_tgt)
+  | hsim_choose_tgt
+      X
+      st_src st_tgt itr_src ktr_tgt
+      fuel f_src f_tgt
+      (SIM: forall x, _hsim hsim Q ctx fuel f_src true (st_src, itr_src) (st_tgt, ktr_tgt x))
+    :
+      _hsim hsim Q ctx fuel f_src f_tgt (st_src, itr_src) (st_tgt, trigger (Choose X) >>= ktr_tgt)
+  | hsim_take_src
+      X
+      st_src st_tgt ktr_src itr_tgt
+      fuel f_src f_tgt
+      (SIM: forall x, _hsim hsim Q ctx None true f_tgt (st_src, ktr_src x) (st_tgt, itr_tgt))
+    :
+      _hsim hsim Q ctx fuel f_src f_tgt (st_src, trigger (Take X) >>= ktr_src) (st_tgt, itr_tgt)
+  | hsim_take_tgt
+      X
+      st_src st_tgt itr_src ktr_tgt
+      fuel f_src f_tgt
+      (SIM: exists x, _hsim hsim Q ctx fuel f_src true (st_src, itr_src) (st_tgt, ktr_tgt x))
+    :
+      _hsim hsim Q ctx fuel f_src f_tgt (st_src, itr_src) (st_tgt, trigger (Take X) >>= ktr_tgt)
+  | hsim_pput_src
+      st_src1
+      st_src0 st_tgt ktr_src itr_tgt
+      fuel f_src f_tgt
+      (SIM: _hsim hsim Q ctx None true f_tgt (st_src1, ktr_src tt) (st_tgt, itr_tgt))
+    :
+      _hsim hsim Q ctx fuel f_src f_tgt (st_src0, trigger (PPut st_src1) >>= ktr_src) (st_tgt, itr_tgt)
+  | hsim_pput_tgt
+      st_tgt1
+      st_src st_tgt0 itr_src ktr_tgt
+      fuel f_src f_tgt
+      (SIM: _hsim hsim Q ctx fuel f_src true (st_src, itr_src) (st_tgt1, ktr_tgt tt))
+    :
+      _hsim hsim Q ctx fuel f_src f_tgt (st_src, itr_src) (st_tgt0, trigger (PPut st_tgt1) >>= ktr_tgt)
+  | hsim_pget_src
+      st_src st_tgt ktr_src itr_tgt
+      fuel f_src f_tgt
+      (SIM: _hsim hsim Q ctx None true f_tgt (st_src, ktr_src st_src) (st_tgt, itr_tgt))
+    :
+      _hsim hsim Q ctx fuel f_src f_tgt (st_src, trigger (PGet) >>= ktr_src) (st_tgt, itr_tgt)
+  | hsim_pget_tgt
+      st_src st_tgt itr_src ktr_tgt
+      fuel f_src f_tgt
+      (SIM: _hsim hsim Q ctx fuel f_src true (st_src, itr_src) (st_tgt, ktr_tgt st_tgt))
+    :
+      _hsim hsim Q ctx fuel f_src f_tgt (st_src, itr_src) (st_tgt, trigger (PGet) >>= ktr_tgt)
+  | hsim_progress
+      st_src st_tgt itr_src itr_tgt
+      fuel
+      (SIM: hsim _ _ Q ctx fuel false false (st_src, itr_src) (st_tgt, itr_tgt))
+    :
+      _hsim hsim Q ctx fuel true true (st_src, itr_src) (st_tgt, itr_tgt)
+  .
+
+  Lemma _hsim_ind2
+        (hsim: forall R_src R_tgt
+                      (Q: Any.t -> Any.t -> R_src -> R_tgt -> iProp)
+                      (ctx: Σ),
+            option ord -> bool -> bool -> Any.t * itree hEs R_src -> Any.t * itree Es R_tgt -> Prop)
+        R_src R_tgt Q ctx
+        (P: option ord -> bool -> bool -> Any.t * itree hEs R_src -> Any.t * itree Es R_tgt -> Prop)
+        (RET: forall
+            v_src v_tgt
+            st_src st_tgt
+            fuel f_src f_tgt
+            (RET: current_iProp ctx (Q st_src st_tgt v_src v_tgt)),
+            P fuel f_src f_tgt (st_src, (Ret v_src)) (st_tgt, (Ret v_tgt)))
+        (CALL: forall
+            fsp (x: fsp.(meta)) w0 FR
+            fn arg_src arg_tgt
+            st_src0 st_tgt0 ktr_src ktr_tgt
+            fuel f_src f_tgt
+            (SPEC: stb fn = Some fsp)
+            (PRE: current_iProp ctx (FR ** I w0 st_src0 st_tgt0 ** fsp.(precond) (Some mn) x arg_src arg_tgt))
+            (MEASURE: o = ord_top)
+            (POST: forall ctx1 w1 st_src1 st_tgt1 ret_src ret_tgt
+                          (ACC: current_iProp ctx1 (FR ** I w1 st_src1 st_tgt1 ** fsp.(postcond) (Some mn) x ret_src ret_tgt)),
+                hsim _ _ Q ctx1 None true true (st_src1, ktr_src ret_src) (st_tgt1, ktr_tgt ret_tgt)),
+            P fuel f_src f_tgt (st_src0, trigger (Call fn arg_src) >>= ktr_src) (st_tgt0, trigger (Call fn arg_tgt) >>= ktr_tgt))
+        (APCSTART: forall
+            fuel1
+            st_src st_tgt ktr_src itr_tgt
+            fuel f_src f_tgt
+            (SIM: _hsim hsim Q ctx (Some (ord_pure fuel1)) true f_tgt (st_src, ktr_src tt) (st_tgt, itr_tgt))
+            (IH: P (Some (ord_pure fuel1)) true f_tgt (st_src, ktr_src tt) (st_tgt, itr_tgt)),
+            P fuel f_src f_tgt (st_src, trigger (hAPC) >>= ktr_src) (st_tgt, itr_tgt))
+        (APCSTEP: forall
+            fsp (x: fsp.(meta)) w0 FR arg_src
+            fn arg_tgt
+            st_src0 st_tgt0 itr_src ktr_tgt
+            fuel0 f_src f_tgt
+            (SPEC: stb fn = Some fsp)
+            (PRE: current_iProp ctx (FR ** I w0 st_src0 st_tgt0 ** fsp.(precond) (Some mn) x arg_src arg_tgt))
+            (MEASURE: ord_lt (fsp.(measure) x) o)
+            (POST: exists fuel1,
+                (<<FUEL: ord_lt fuel1 fuel0>>) /\
+                (<<SIM: forall ctx1 w1 st_src1 st_tgt1 ret_src ret_tgt
+                               (ACC: current_iProp ctx1 (FR ** I w1 st_src1 st_tgt1 ** fsp.(postcond) (Some mn) x ret_src ret_tgt)),
+                    hsim _ _ Q ctx1 (Some fuel1) true true (st_src1, itr_src) (st_tgt1, ktr_tgt ret_tgt)>>)),
+            P (Some fuel0) f_src f_tgt (st_src0, itr_src) (st_tgt0, trigger (Call fn arg_tgt) >>= ktr_tgt))
+        (SYSCALL: forall
+            fn arg rvs
+            st_src st_tgt ktr_src ktr_tgt
+            fuel f_src f_tgt
+            (POST: forall ret,
+                hsim _ _ Q ctx None true true (st_src, ktr_src ret) (st_tgt, ktr_tgt ret)),
+            P fuel f_src f_tgt (st_src, trigger (Syscall fn arg rvs) >>= ktr_src) (st_tgt, trigger (Syscall fn arg rvs) >>= ktr_tgt))
+        (TAUSRC: forall
+            st_src st_tgt itr_src itr_tgt
+            fuel f_src f_tgt
+            (SIM: _hsim hsim Q ctx None true f_tgt (st_src, itr_src) (st_tgt, itr_tgt))
+            (IH: P None true f_tgt (st_src, itr_src) (st_tgt, itr_tgt))
+          ,
+            P fuel f_src f_tgt (st_src, tau;; itr_src) (st_tgt, itr_tgt))
+        (TAUTGT: forall
+            st_src st_tgt itr_src itr_tgt
+            fuel f_src f_tgt
+            (SIM: _hsim hsim Q ctx fuel f_src true (st_src, itr_src) (st_tgt, itr_tgt))
+            (IH: P fuel f_src true (st_src, itr_src) (st_tgt, itr_tgt)),
+            P fuel f_src f_tgt (st_src, itr_src) (st_tgt, tau;; itr_tgt))
+        (CHOOSESRC: forall
+            X
+            st_src st_tgt ktr_src itr_tgt
+            fuel f_src f_tgt
+            (SIM: exists x, (<<SIM: _hsim hsim Q ctx None true f_tgt (st_src, ktr_src x) (st_tgt, itr_tgt)>>) /\ (<<IH: P None true f_tgt (st_src, ktr_src x) (st_tgt, itr_tgt)>>)),
+            P fuel f_src f_tgt (st_src, trigger (Choose X) >>= ktr_src) (st_tgt, itr_tgt))
+        (CHOOSETGT: forall
+            X
+            st_src st_tgt itr_src ktr_tgt
+            fuel f_src f_tgt
+            (SIM: forall x, (<<SIM: _hsim hsim Q ctx fuel f_src true (st_src, itr_src) (st_tgt, ktr_tgt x)>>) /\ (<<IH: P fuel f_src true (st_src, itr_src) (st_tgt, ktr_tgt x)>>)),
+            P fuel f_src f_tgt (st_src, itr_src) (st_tgt, trigger (Choose X) >>= ktr_tgt))
+        (TAKESRC: forall
+            X
+            st_src st_tgt ktr_src itr_tgt
+            fuel f_src f_tgt
+            (SIM: forall x, (<<SIM: _hsim hsim Q ctx None true f_tgt (st_src, ktr_src x) (st_tgt, itr_tgt)>>) /\ (<<IH: P None true f_tgt (st_src, ktr_src x) (st_tgt, itr_tgt)>>)),
+            P fuel f_src f_tgt (st_src, trigger (Take X) >>= ktr_src) (st_tgt, itr_tgt))
+        (TAKETGT: forall
+            X
+            st_src st_tgt itr_src ktr_tgt
+            fuel f_src f_tgt
+            (SIM: exists x, (<<SIM: _hsim hsim Q ctx fuel f_src true (st_src, itr_src) (st_tgt, ktr_tgt x)>>) /\ (<<IH: P fuel f_src true (st_src, itr_src) (st_tgt, ktr_tgt x)>>)),
+            P fuel f_src f_tgt (st_src, itr_src) (st_tgt, trigger (Take X) >>= ktr_tgt))
+        (PPUTSRC: forall
+            st_src1
+            st_src0 st_tgt ktr_src itr_tgt
+            fuel f_src f_tgt
+            (SIM: _hsim hsim Q ctx None true f_tgt (st_src1, ktr_src tt) (st_tgt, itr_tgt))
+            (IH: P None true f_tgt (st_src1, ktr_src tt) (st_tgt, itr_tgt)),
+            P fuel f_src f_tgt (st_src0, trigger (PPut st_src1) >>= ktr_src) (st_tgt, itr_tgt))
+        (PPUTTGT: forall
+            st_tgt1
+            st_src st_tgt0 itr_src ktr_tgt
+            fuel f_src f_tgt
+            (SIM: _hsim hsim Q ctx fuel f_src true (st_src, itr_src) (st_tgt1, ktr_tgt tt))
+            (IH: P fuel f_src true (st_src, itr_src) (st_tgt1, ktr_tgt tt)),
+            P fuel f_src f_tgt (st_src, itr_src) (st_tgt0, trigger (PPut st_tgt1) >>= ktr_tgt))
+        (PGETSRC: forall
+            st_src st_tgt ktr_src itr_tgt
+            fuel f_src f_tgt
+            (SIM: _hsim hsim Q ctx None true f_tgt (st_src, ktr_src st_src) (st_tgt, itr_tgt))
+            (IH: P None true f_tgt (st_src, ktr_src st_src) (st_tgt, itr_tgt)),
+            P fuel f_src f_tgt (st_src, trigger (PGet) >>= ktr_src) (st_tgt, itr_tgt))
+        (PGETTGT: forall
+            st_src st_tgt itr_src ktr_tgt
+            fuel f_src f_tgt
+            (SIM: _hsim hsim Q ctx fuel f_src true (st_src, itr_src) (st_tgt, ktr_tgt st_tgt))
+            (IH: P fuel f_src true (st_src, itr_src) (st_tgt, ktr_tgt st_tgt)),
+            P fuel f_src f_tgt (st_src, itr_src) (st_tgt, trigger (PGet) >>= ktr_tgt))
+        (PROGRESS: forall
+            st_src st_tgt itr_src itr_tgt
+            fuel
+            (SIM: hsim _ _ Q ctx fuel false false (st_src, itr_src) (st_tgt, itr_tgt)),
+            P fuel true true (st_src, itr_src) (st_tgt, itr_tgt))
+    :
+      forall fuel f_src f_tgt st_src st_tgt
+             (SIM: @_hsim hsim _ _ Q ctx fuel f_src f_tgt st_src st_tgt),
+        P fuel f_src f_tgt st_src st_tgt.
+  Proof.
+    fix IH 6. i. inv SIM.
+    { eapply RET; eauto. }
+    { eapply CALL; eauto. }
+    { eapply APCSTART; eauto. }
+    { des. eapply APCSTEP; eauto. }
+    { eapply SYSCALL; eauto. }
+    { eapply TAUSRC; eauto. }
+    { eapply TAUTGT; eauto. }
+    { des. eapply CHOOSESRC; eauto. }
+    { eapply CHOOSETGT; eauto. }
+    { eapply TAKESRC; eauto. }
+    { des. eapply TAKETGT; eauto. }
+    { eapply PPUTSRC; eauto. }
+    { eapply PPUTTGT; eauto. }
+    { eapply PGETSRC; eauto. }
+    { eapply PGETTGT; eauto. }
+    { eapply PROGRESS; eauto. }
+  Qed.
+
+  Definition hsim := paco9 _hsim bot9.
+  Arguments hsim [_ _] _ _ _ _ _ _ _.
+
+  Lemma _hsim_mon: monotone9 _hsim.
+  Proof.
+    ii. induction IN using _hsim_ind2.
+    { econs 1; eauto. }
+    { econs 2; eauto. }
+    { econs 3; eauto. }
+    { des. econs 4; eauto. esplits; eauto. }
+    { econs 5; eauto. }
+    { econs 6; eauto. }
+    { econs 7; eauto. }
+    { econs 8; eauto. des. esplits; eauto. }
+    { econs 9; eauto. i. hexploit SIM; eauto. i. des. eauto. }
+    { econs 10; eauto. i. hexploit SIM; eauto. i. des. eauto. }
+    { econs 11; eauto. des. esplits; eauto. }
+    { econs 12; eauto. }
+    { econs 13; eauto. }
+    { econs 14; eauto. }
+    { econs 15; eauto. }
+    { econs 16; eauto. }
+  Qed.
+  Hint Resolve _hsim_mon: paco.
+
+  Lemma hsim_ind
+        R_src R_tgt Q ctx
+        (P: option ord -> bool -> bool -> Any.t * itree hEs R_src -> Any.t * itree Es R_tgt -> Prop)
+        (RET: forall
+            v_src v_tgt
+            st_src st_tgt
+            fuel f_src f_tgt
+            (RET: current_iProp ctx (Q st_src st_tgt v_src v_tgt)),
+            P fuel f_src f_tgt (st_src, (Ret v_src)) (st_tgt, (Ret v_tgt)))
+        (CALL: forall
+            fsp (x: fsp.(meta)) w0 FR
+            fn arg_src arg_tgt
+            st_src0 st_tgt0 ktr_src ktr_tgt
+            fuel f_src f_tgt
+            (SPEC: stb fn = Some fsp)
+            (PRE: current_iProp ctx (FR ** I w0 st_src0 st_tgt0 ** fsp.(precond) (Some mn) x arg_src arg_tgt))
+            (MEASURE: o = ord_top)
+            (POST: forall ctx1 w1 st_src1 st_tgt1 ret_src ret_tgt
+                          (ACC: current_iProp ctx1 (FR ** I w1 st_src1 st_tgt1 ** fsp.(postcond) (Some mn) x ret_src ret_tgt)),
+                hsim Q ctx1 None true true (st_src1, ktr_src ret_src) (st_tgt1, ktr_tgt ret_tgt)),
+            P fuel f_src f_tgt (st_src0, trigger (Call fn arg_src) >>= ktr_src) (st_tgt0, trigger (Call fn arg_tgt) >>= ktr_tgt))
+        (APCSTART: forall
+            fuel1
+            st_src st_tgt ktr_src itr_tgt
+            fuel f_src f_tgt
+            (SIM: hsim Q ctx (Some (ord_pure fuel1)) true f_tgt (st_src, ktr_src tt) (st_tgt, itr_tgt))
+            (IH: P (Some (ord_pure fuel1)) true f_tgt (st_src, ktr_src tt) (st_tgt, itr_tgt)),
+            P fuel f_src f_tgt (st_src, trigger (hAPC) >>= ktr_src) (st_tgt, itr_tgt))
+        (APCSTEP: forall
+            fsp (x: fsp.(meta)) w0 FR fuel1 arg_src
+            fn arg_tgt
+            st_src0 st_tgt0 itr_src ktr_tgt
+            fuel0 f_src f_tgt
+            (SPEC: stb fn = Some fsp)
+            (PRE: current_iProp ctx (FR ** I w0 st_src0 st_tgt0 ** fsp.(precond) (Some mn) x arg_src arg_tgt))
+            (FUEL: ord_lt fuel1 fuel0)
+            (POST: forall ctx1 w1 st_src1 st_tgt1 ret_src ret_tgt
+                          (ACC: current_iProp ctx1 (FR ** I w1 st_src1 st_tgt1 ** fsp.(postcond) (Some mn) x ret_src ret_tgt)),
+                hsim Q ctx1 (Some fuel1) true true (st_src1, itr_src) (st_tgt1, ktr_tgt ret_tgt)),
+            P (Some fuel0) f_src f_tgt (st_src0, itr_src) (st_tgt0, trigger (Call fn arg_tgt) >>= ktr_tgt))
+        (SYSCALL: forall
+            fn arg rvs
+            st_src st_tgt ktr_src ktr_tgt
+            fuel f_src f_tgt
+            (POST: forall ret,
+                hsim Q ctx None true true (st_src, ktr_src ret) (st_tgt, ktr_tgt ret)),
+            P fuel f_src f_tgt (st_src, trigger (Syscall fn arg rvs) >>= ktr_src) (st_tgt, trigger (Syscall fn arg rvs) >>= ktr_tgt))
+        (TAUSRC: forall
+            st_src st_tgt itr_src itr_tgt
+            fuel f_src f_tgt
+            (SIM: hsim Q ctx None true f_tgt (st_src, itr_src) (st_tgt, itr_tgt))
+            (IH: P None true f_tgt (st_src, itr_src) (st_tgt, itr_tgt))
+          ,
+            P fuel f_src f_tgt (st_src, tau;; itr_src) (st_tgt, itr_tgt))
+        (TAUTGT: forall
+            st_src st_tgt itr_src itr_tgt
+            fuel f_src f_tgt
+            (SIM: hsim Q ctx fuel f_src true (st_src, itr_src) (st_tgt, itr_tgt))
+            (IH: P fuel f_src true (st_src, itr_src) (st_tgt, itr_tgt)),
+            P fuel f_src f_tgt (st_src, itr_src) (st_tgt, tau;; itr_tgt))
+        (CHOOSESRC: forall
+            X
+            st_src st_tgt ktr_src itr_tgt
+            fuel f_src f_tgt
+            (SIM: exists x, (<<SIM: hsim Q ctx None true f_tgt (st_src, ktr_src x) (st_tgt, itr_tgt)>>) /\ (<<IH: P None true f_tgt (st_src, ktr_src x) (st_tgt, itr_tgt)>>)),
+            P fuel f_src f_tgt (st_src, trigger (Choose X) >>= ktr_src) (st_tgt, itr_tgt))
+        (CHOOSETGT: forall
+            X
+            st_src st_tgt itr_src ktr_tgt
+            fuel f_src f_tgt
+            (SIM: forall x, (<<SIM: hsim Q ctx fuel f_src true (st_src, itr_src) (st_tgt, ktr_tgt x)>>) /\ (<<IH: P fuel f_src true (st_src, itr_src) (st_tgt, ktr_tgt x)>>)),
+            P fuel f_src f_tgt (st_src, itr_src) (st_tgt, trigger (Choose X) >>= ktr_tgt))
+        (TAKESRC: forall
+            X
+            st_src st_tgt ktr_src itr_tgt
+            fuel f_src f_tgt
+            (SIM: forall x, (<<SIM: hsim Q ctx None true f_tgt (st_src, ktr_src x) (st_tgt, itr_tgt)>>) /\ (<<IH: P None true f_tgt (st_src, ktr_src x) (st_tgt, itr_tgt)>>)),
+            P fuel f_src f_tgt (st_src, trigger (Take X) >>= ktr_src) (st_tgt, itr_tgt))
+        (TAKETGT: forall
+            X
+            st_src st_tgt itr_src ktr_tgt
+            fuel f_src f_tgt
+            (SIM: exists x, (<<SIM: hsim Q ctx fuel f_src true (st_src, itr_src) (st_tgt, ktr_tgt x)>>) /\ (<<IH: P fuel f_src true (st_src, itr_src) (st_tgt, ktr_tgt x)>>)),
+            P fuel f_src f_tgt (st_src, itr_src) (st_tgt, trigger (Take X) >>= ktr_tgt))
+        (PPUTSRC: forall
+            st_src1
+            st_src0 st_tgt ktr_src itr_tgt
+            fuel f_src f_tgt
+            (SIM: hsim Q ctx None true f_tgt (st_src1, ktr_src tt) (st_tgt, itr_tgt))
+            (IH: P None true f_tgt (st_src1, ktr_src tt) (st_tgt, itr_tgt)),
+            P fuel f_src f_tgt (st_src0, trigger (PPut st_src1) >>= ktr_src) (st_tgt, itr_tgt))
+        (PPUTTGT: forall
+            st_tgt1
+            st_src st_tgt0 itr_src ktr_tgt
+            fuel f_src f_tgt
+            (SIM: hsim Q ctx fuel f_src true (st_src, itr_src) (st_tgt1, ktr_tgt tt))
+            (IH: P fuel f_src true (st_src, itr_src) (st_tgt1, ktr_tgt tt)),
+            P fuel f_src f_tgt (st_src, itr_src) (st_tgt0, trigger (PPut st_tgt1) >>= ktr_tgt))
+        (PGETSRC: forall
+            st_src st_tgt ktr_src itr_tgt
+            fuel f_src f_tgt
+            (SIM: hsim Q ctx None true f_tgt (st_src, ktr_src st_src) (st_tgt, itr_tgt))
+            (IH: P None true f_tgt (st_src, ktr_src st_src) (st_tgt, itr_tgt)),
+            P fuel f_src f_tgt (st_src, trigger (PGet) >>= ktr_src) (st_tgt, itr_tgt))
+        (PGETTGT: forall
+            st_src st_tgt itr_src ktr_tgt
+            fuel f_src f_tgt
+            (SIM: hsim Q ctx fuel f_src true (st_src, itr_src) (st_tgt, ktr_tgt st_tgt))
+            (IH: P fuel f_src true (st_src, itr_src) (st_tgt, ktr_tgt st_tgt)),
+            P fuel f_src f_tgt (st_src, itr_src) (st_tgt, trigger (PGet) >>= ktr_tgt))
+        (PROGRESS: forall
+            st_src st_tgt itr_src itr_tgt
+            fuel
+            (SIM: hsim Q ctx fuel false false (st_src, itr_src) (st_tgt, itr_tgt)),
+            P fuel true true (st_src, itr_src) (st_tgt, itr_tgt))
+    :
+      forall fuel f_src f_tgt st_src st_tgt
+             (SIM: hsim Q ctx fuel f_src f_tgt st_src st_tgt),
+        P fuel f_src f_tgt st_src st_tgt.
+  Proof.
+    i. punfold SIM. induction SIM using _hsim_ind2.
+    { eapply RET; eauto. }
+    { eapply CALL; eauto. i. hexploit POST; eauto. i. pclearbot. eauto. }
+    { eapply APCSTART; eauto. pfold. eauto. }
+    { des. eapply APCSTEP; eauto. i. hexploit SIM; eauto. i. pclearbot. eauto. }
+    { eapply SYSCALL; eauto. i. hexploit POST; eauto. i. pclearbot. eauto. }
+    { eapply TAUSRC; eauto. pfold. eauto. }
+    { eapply TAUTGT; eauto. pfold. eauto. }
+    { des. eapply CHOOSESRC; eauto. esplits; eauto. pfold. eauto. }
+    { eapply CHOOSETGT; eauto. i. hexploit SIM; eauto. i. des. pclearbot. splits; eauto. pfold. eauto. }
+    { eapply TAKESRC; eauto. i. hexploit SIM; eauto. i. des. pclearbot. splits; eauto. pfold. eauto. }
+    { des. eapply TAKETGT; eauto. esplits; eauto. pfold. eauto. }
+    { eapply PPUTSRC; eauto. pfold. eauto. }
+    { eapply PPUTTGT; eauto. pfold. eauto. }
+    { eapply PGETSRC; eauto. pfold. eauto. }
+    { eapply PGETTGT; eauto. pfold. eauto. }
+    { eapply PROGRESS; eauto. pclearbot. eauto. }
+  Qed.
+
+  Variant myr w0:
+    bool -> bool -> world → Any.t * itree Es Any.t → Any.t * itree Es Any.t → Prop :=
+  | myr_intro0
+      f_src f_tgt st_src st_tgt (itr_src: itree (hAPCE +' Es) Any.t) itr_tgt mr_src ctx X (x: X) Q mn_caller
+      (SIM: hsim (fun st_src st_tgt ret_src ret_tgt =>
+                    (∃ w1, ⌜le w0 w1⌝ ** I w1 st_src st_tgt) ** (Q mn_caller x ret_src ret_tgt: iProp)) ctx None f_src f_tgt (st_src, itr_src) (st_tgt, itr_tgt))
+    :
+      @myr
+        w0
+        f_src f_tgt w0
+        (Any.pair st_src mr_src, (interp_hCallE_tgt mn stb o (interp_hEs_tgt itr_src) ctx) >>= (HoareFunRet Q mn_caller x))
+        (st_tgt, itr_tgt)
+  | myr_intro1
+      fuel f_src f_tgt st_src st_tgt (itr_src: itree (hAPCE +' Es) Any.t)  itr_tgt mr_src ctx X (x: X) Q mn_caller at_most
+      (SIM: hsim (fun st_src st_tgt ret_src ret_tgt =>
+                    (∃ w1, ⌜le w0 w1⌝ ** I w1 st_src st_tgt) ** (Q mn_caller x ret_src ret_tgt: iProp)) ctx (Some (ord_pure fuel)) f_src f_tgt (st_src, itr_src) (st_tgt, itr_tgt))
+    :
+      @myr
+        w0
+        f_src f_tgt w0
+        (Any.pair st_src mr_src,
+         '(ctx0, _) <- (interp_hCallE_tgt mn stb o (_APC at_most) ctx);;
+         (interp_hCallE_tgt mn stb o (interp_hEs_tgt itr_src) ctx0) >>= (HoareFunRet Q mn_caller x))
+        (st_tgt, itr_tgt)
+  .
+
+  Lemma current_iPropL_convert ctx P
+        (CUR: current_iProp ctx P)
+    :
+      current_iPropL ctx [("H", P)].
+  Proof.
+    unfold current_iPropL. ss. unfold from_iPropL.
+    eapply current_iProp_entail; eauto.
+  Qed.
+
+  Lemma hsim_adequacy_aux w0:
+    myr w0 <5= paco8 (_sim_itree (mk_wf I) le) bot8 Any.t Any.t (lift_rel (mk_wf I) le w0 (@eq Any.t)).
+  Proof.
+    ginit. gcofix CIH. i. inv PR.
+    { remember (st_src, itr_src). remember (st_tgt, itr_tgt). remember None.
+      revert st_src st_tgt itr_src itr_tgt Heqp Heqp0 Heqo0.
+      induction SIM using hsim_ind; i; clarify.
+      { steps. eapply current_iPropL_convert in RET.
+        mDesAll. hret _; eauto. iModIntro. iSplitL "A1"; auto.
+      }
+      { eapply current_iPropL_convert in PRE. mDesAll. steps.
+        rewrite SPEC. steps. destruct fsp. ss. hcall _ _ with "A A1".
+        { iModIntro. iSplitL "A1"; eauto. iApply "A". }
+        { rewrite MEASURE in *. splits; ss.
+          { unfold ord_lt. des_ifs. }
+          { admit "". }
+        }
+        { steps. gbase. eapply CIH. left. eapply POST; eauto. admit "". }
+      }
+      { steps. admit "". }
+      { steps. gbase. eapply CIH. left. auto. }
+      { steps. eapply IHSIM; eauto. }
+      { steps. eapply IHSIM; eauto. }
+      { des. steps. force_l. esplits. steps. eapply IH; eauto. }
+      { steps. hexploit SIM; eauto. i. des. eapply IH; eauto. }
+      { steps. hexploit SIM; eauto. i. des. eapply IH; eauto. }
+      { des. steps. force_r. esplits. steps. eapply IH; eauto. }
+      { steps. eapply IHSIM; eauto. }
+      { steps. eapply IHSIM; eauto. }
+      { steps. eapply IHSIM; eauto. }
+      { steps. eapply IHSIM; eauto. }
+      { deflag. gbase. eapply CIH. left. auto. }
+    }
+    { revert x8 x9 fuel st_src st_tgt itr_src itr_tgt mr_src ctx X x Q mn_caller SIM.
+      induction (Ord.lt_well_founded at_most).
+      clear H. rename x into at_most. rename H0 into IH. i.
+      induction SIM using hsim_ind; i; clarify.
+      { astop. eapply IH.
+
+steps. eapply current_iPropL_convert in RET.
+        mDesAll. astop. steps. hret _; eauto. iModIntro. iSplitL "A1"; auto.
+      }
+      { eapply current_iPropL_convert in PRE. mDesAll. steps.
+        rewrite SPEC. steps. destruct fsp. ss. hcall _ _ with "A A1".
+        { iModIntro. iSplitL "A1"; eauto. iApply "A". }
+        { rewrite MEASURE in *. splits; ss.
+          { unfold ord_lt. des_ifs. }
+          { admit "". }
+        }
+        { steps. gbase. eapply CIH. left. eapply POST; eauto. admit "". }
+      }
+      { steps. admit "". }
+      { steps. gbase. eapply CIH. left. auto. }
+      { steps. eapply IHSIM; eauto. }
+      { steps. eapply IHSIM; eauto. }
+      { des. steps. force_l. esplits. steps. eapply IH; eauto. }
+      { steps. hexploit SIM; eauto. i. des. eapply IH; eauto. }
+      { steps. hexploit SIM; eauto. i. des. eapply IH; eauto. }
+      { des. steps. force_r. esplits. steps. eapply IH; eauto. }
+      { steps. eapply IHSIM; eauto. }
+      { steps. eapply IHSIM; eauto. }
+      { steps. eapply IHSIM; eauto. }
+      { steps. eapply IHSIM; eauto. }
+      { deflag. gbase. eapply CIH. left. auto. }
+      { astop.
+
+    }
+    }
+
+
+eapply SIM; eauto. steps. eapply IHSIM; eauto. }
+
+
+
+          eapply current
+
+gstep.
+
+admit "". }
+}
+
+
+destruct (measure x0); auto. econs.
+
+clarif
+
+eapply hcall_clo.
+
+
+        hcall _ _ with "A A1".
+
+auto.
+
+
+        cut ((current_iPropL ctx [("H0", ((∃ w1 : world, ⌜le x10 w1⌝ ** I w1 st_src0 st_tgt0) ** Q mn_caller x v_src v_tgt))])).
+
+        change (current_iProp ctx
+                              ((∃ w1 : world, ⌜le x10 w1⌝ ** I w1 st_src0 st_tgt0) **
+                                                                                   Q mn_caller x v_src v_tgt)) with (current_iPropL ctx [("H0", ((∃ w1 : world, ⌜le x10 w1⌝ ** I w1 st_src0 st_tgt0) **
+                                                                                                                                                                                                     Q mn_caller x v_src v_tgt))]) in RET.
+
+
+iPropL
+current_iPropL eapply hret_clo. hret _.
+
+
+induction SIM
+
+
+
+
+    forall fuel f_src f_tgt st_src st_tgt (itr_src: itree (hAPCE +' Es) Any.t)  itr_tgt mr_src ctx w0 X (x: X) Q mn_caller
+           (SIM: hsim (fun st_src st_tgt ret_src ret_tgt =>
+                         (∃ w1, ⌜le w0 w1⌝ ** I w1 st_src st_tgt) ** (Q mn_caller x ret_src ret_tgt: iProp)) ctx fuel f_src f_tgt (st_src, itr_src) (st_tgt, itr_tgt)),
+      paco8 (_sim_itree (mk_wf I) le) bot8
+            Any.t Any.t
+            (lift_rel (mk_wf I) le w0 (@eq Any.t))
+            f_src f_tgt w0
+            (Any.pair st_src mr_src, (interp_hCallE_tgt mn stb o (interp_hEs_tgt itr_src) ctx) >>= (HoareFunRet Q mn_caller x))
+            (st_tgt, itr_tgt).
+  Proof.
+    ginit. gcofix CIH. i.
+
+  Lemma hsim_adequacy:
+    forall fuel f_src f_tgt st_src st_tgt (itr_src: itree (hAPCE +' Es) Any.t)  itr_tgt mr_src ctx w0 X (x: X) Q mn_caller
+           (SIM: hsim (fun st_src st_tgt ret_src ret_tgt =>
+                         (∃ w1, ⌜le w0 w1⌝ ** I w1 st_src st_tgt) ** (Q mn_caller x ret_src ret_tgt: iProp)) ctx fuel f_src f_tgt (st_src, itr_src) (st_tgt, itr_tgt)),
+      paco8 (_sim_itree (mk_wf I) le) bot8
+            Any.t Any.t
+            (lift_rel (mk_wf I) le w0 (@eq Any.t))
+            f_src f_tgt w0
+            (Any.pair st_src mr_src, (interp_hCallE_tgt mn stb o (interp_hEs_tgt itr_src) ctx) >>= (HoareFunRet Q mn_caller x))
+            (st_tgt, itr_tgt).
+  Proof.
+    ginit. gcofix CIH. i.
+
+
+
+
+HoareFun
+    Es'
+
+    (Q: Any.t -> Any.t -> R_src -> R_tgt -> iProp)
+
+      (fun st_src st_tgt ret_src ret_tgt =>
+         (∃ w1, ⌜le w0 w1⌝ ** I w1 st_src st_tgt) ** (Q mn x ret_src ret_tgt: iProp))
+
+
+        (UPDATABLE:
+           (from_iPropL l) ⊢ #=> (R a mp_src mp_tgt ** (Q mn x vret_src vret_tgt: iProp)))
+
+        (EQ: forall (mr_src1: Σ) (WLE: le a0 a) (WF: mk_wf R a (Any.pair mp_src mr_src1↑, mp_tgt)),
+            eqr (Any.pair mp_src mr_src1↑) mp_tgt vret_tgt vret_tgt)
+
+
+
+(lift_rel (mk_wf wf) le w0
+
+
+         (fun
+(lift_rel wf le w0 eq)
+
+    ((∃ ) ** Q)
+
+    (fun lift_rel
+
+            (Q: Any.t -> Any.t -> R_src -> R_tgt -> iProp)
+
+
+sim_itree =
+λ (st_local := Any.t) (world : Type) (W := (Any.t * Any.t)%type)
+  (wf : world → W → Prop) (le : relation world) (o_src o_tgt : bool)
+  (w0 : world),
+  paco8 (_sim_itree wf le) bot8 Any.t Any.t (lift_rel wf le w0 eq) o_src o_tgt w0
+     : ∀ world : Type,
+         (world → Any.t * Any.t → Prop)
+         → relation world → bool → bool → world → relation (Any.t * itree Es Any.t)
+
+
+sim_itree
+        (WLE: le a0 a)
+
+        (UPDATABLE:
+           (from_iPropL l) ⊢ #=> (R a mp_src mp_tgt ** (Q mn x vret_src vret_tgt: iProp)))
+
+
+             (Any.pair mp_src mr_src, (HoareFunRet Q mn x (ctx, vret_src)))
+
+
+    interp_
+
+
+      (POST: gpaco8 (_sim_itree wf le) (cpn8 (_sim_itree wf le)) r rg _ _ eqr true n a
+                    (st_src,
+                     (interp_hCallE_tgt mn stb o itr_src ctx) >>= HoareFunRet )
+                    (itr_tgt))
+
+
+        P fuel f_src f_tgt st_src st_tgt.
+
+    forall fuel
+
+
+Variant hCallE: Type -> Type :=
+| hCall (tbr: bool) (fn: gname) (varg_src: Any_src): hCallE Any_src
+(*** tbr == to be removed ***)
+.
+
+Variant hAPCE: Type -> Type :=
+| hAPC: hAPCE unit
+.
+
+
+  | hsim_call
+      f_src f_tgt ctx st_src0 st_tgt0 w0
+      v_src v_tgt
+      (RET: current_iProp ctx (Q st_src0 st_tgt0 v_src v_tgt))
+
+
+    :
+      @_hsim r R_src R_tgt Q ctx f_src f_tgt (st_src0, (Ret v_src)) (st_tgt0, (Ret v_tgt))
+  .
+
+  | hsim_
+      i_src0 i_tgt0 w0 st_src0 st_tgt0
+      v_src v_tgt
+      (RET: current_iProp ctx (Q st_src0 st_tgt0 v_src v_tgt))
+    :
+      _hsim r Q ctx i_src0 i_tgt0 w0 (st_src0, (Ret v_src)) (st_tgt0, (Ret v_tgt))
+  .
+
+RR i_src0 i_tgt0 w0 (st_src0, (Ret v_src)) (st_tgt0, (Ret v_tgt))
+  .
+
+  | safe_sim_itree_call
+      i_src0 i_tgt0 w st_src0 st_tgt0
+      fn varg k_src k_tgt
+      (SIM: exists w0,
+          (<<WF: wf w0 (st_src0, st_tgt0)>>) /\
+          (<<K: forall w1 vret st_src1 st_tgt1 (WLE: le w0 w1) (WF: wf w1 (st_src1, st_tgt1)),
+              g _ _ RR true true w (st_src1, k_src vret) (st_tgt1, k_tgt vret)>>))
+    :
+      _safe_sim_itree r g RR i_src0 i_tgt0 w (st_src0, trigger (Call fn varg) >>= k_src)
+                      (st_tgt0, trigger (Call fn varg) >>= k_tgt)
+
+  | safe_sim_itree_syscall
+      i_src0 i_tgt0 w0 st_src0 st_tgt0
+      fn varg rvs k_src k_tgt
+      (K: forall vret,
+          g _ _ RR true true w0 (st_src0, k_src vret) (st_tgt0, k_tgt vret))
+    :
+      _safe_sim_itree r g RR i_src0 i_tgt0 w0 (st_src0, trigger (Syscall fn varg rvs) >>= k_src)
+                      (st_tgt0, trigger (Syscall fn varg rvs) >>= k_tgt)
+
+  | safe_sim_itree_tau_src
+      i_src0 i_tgt0 w0 st_src0 st_tgt0
+      i_src i_tgt
+      (K: r _ _ RR true i_tgt0 w0 (st_src0, i_src) (st_tgt0, i_tgt))
+    :
+      _safe_sim_itree r g RR i_src0 i_tgt0 w0 (st_src0, tau;; i_src) (st_tgt0, i_tgt)
+  | safe_sim_itree_take_src
+      i_src0 i_tgt0 w0 st_src0 st_tgt0
+      X k_src i_tgt
+      (K: forall (x: X), r _ _ RR true i_tgt0 w0 (st_src0, k_src x) (st_tgt0, i_tgt))
+    :
+      _safe_sim_itree r g RR i_src0 i_tgt0 w0 (st_src0, trigger (Take X) >>= k_src)
+                      (st_tgt0, i_tgt)
+
+  | safe_sim_itree_pput_src
+      i_src0 i_tgt0 w0 st_tgt0 st_src0
+      k_src i_tgt
+      st_src1
+      (K: r _ _ RR true i_tgt0 w0 (st_src1, k_src tt) (st_tgt0, i_tgt))
+    :
+      _safe_sim_itree r g RR i_src0 i_tgt0 w0 (st_src0, trigger (PPut st_src1) >>= k_src)
+                      (st_tgt0, i_tgt)
+
+  | safe_sim_itree_pget_src
+      i_src0 i_tgt0 w0 st_tgt0 st_src0
+      k_src i_tgt
+      (K: r _ _ RR true i_tgt0 w0 (st_src0, k_src st_src0) (st_tgt0, i_tgt))
+    :
+      _safe_sim_itree r g RR i_src0 i_tgt0 w0 (st_src0, trigger (PGet) >>= k_src)
+                      (st_tgt0, i_tgt)
+
+
+  | safe_sim_itree_tau_tgt
+      i_src0 i_tgt0 w0 st_src0 st_tgt0
+      i_src i_tgt
+      (K: r _ _ RR i_src0 true w0 (st_src0, i_src) (st_tgt0, i_tgt))
+    :
+      _safe_sim_itree r g RR i_src0 i_tgt0 w0 (st_src0, i_src) (st_tgt0, tau;; i_tgt)
+  | safe_sim_itree_choose_tgt
+      i_src0 i_tgt0 w0 st_src0 st_tgt0
+      X i_src k_tgt
+      (K: forall (x: X), r _ _ RR i_src0 true w0 (st_src0, i_src) (st_tgt0, k_tgt x))
+    :
+      _safe_sim_itree r g RR i_src0 i_tgt0 w0 (st_src0, i_src)
+                      (st_tgt0, trigger (Choose X) >>= k_tgt)
+
+  | safe_sim_itree_pput_tgt
+      i_src0 i_tgt0 w0 st_src0 st_tgt0
+      k_tgt i_src
+      st_tgt1
+      (K: r _ _ RR i_src0 true w0 (st_src0, i_src) (st_tgt1, k_tgt tt))
+    :
+      _safe_sim_itree r g RR i_src0 i_tgt0 w0 (st_src0, i_src)
+                      (st_tgt0, trigger (PPut st_tgt1) >>= k_tgt)
+
+  | safe_sim_itree_pget_tgt
+      i_src0 i_tgt0 w0 st_src0 st_tgt0
+      k_tgt i_src
+      (K: r _ _ RR i_src0 true w0 (st_src0, i_src) (st_tgt0, k_tgt st_tgt0))
+    :
+      _safe_sim_itree r g RR i_src0 i_tgt0 w0 (st_src0, i_src)
+                      (st_tgt0, trigger (PGet) >>= k_tgt)
+  .
+
+  Lemma safe_sim_sim r g:
+    @_safe_sim_itree (gpaco8 (_sim_itree wf le) (cpn8 (_sim_itree wf le)) r g) (gpaco8 (_sim_itree wf le) (cpn8 (_sim_itree wf le)) g g)
+    <8=
+    gpaco8 (_sim_itree wf le) (cpn8 (_sim_itree wf le)) r g.
+  Proof.
+    i. eapply sim_itreeC_spec. inv PR; try by (econs; eauto).
+    des. econs; eauto.
+  Qed.
+
+End SIM.
+
+
+Section HLEMMAS.
+  Context `{Σ: GRA.t}.
+  Local Opaque GRA.to_URA.
+
+  Variant mk_wf (A: Type)
+          (R: A -> Any.t -> Any.t -> iProp)
+    : A -> Any.t * Any.t -> Prop :=
+  | mk_wf_intro
+      a
+      mr_src mp_src mp_tgt
+      (RSRC: URA.wf mr_src -> R a mp_src mp_tgt mr_src)
+    :
+      mk_wf R a ((Any.pair mp_src mr_src↑), mp_tgt)
+  .
+
+  Definition inv_wf
+             `{@GRA.inG invRA Σ}
+             A
+             (R: A -> Any.t -> Any.t -> iProp)
+    : _ -> (Any.t * Any.t -> Prop) :=
+    @mk_wf
+      (A + Any.t * Any.t)%type
+      (fun a' mp_src mp_tgt =>
+         match a' with
+         | inl a => R a mp_src mp_tgt
+         | inr (mp_src1, mp_tgt1) => inv_closed ** ⌜mp_src1 = mp_src /\ mp_tgt1 = mp_tgt⌝
+         end)%I
+  .
+
+  Lemma hcall_clo_ord_weaken'
+        (fsp1: fspec)
+        (x: shelve__ fsp1.(meta))
+
+        A (a0: shelve__ A) FR
+
+        (le: A -> A -> Prop) mn r rg a n m mr_src0 mp_src0
+        (fsp0: fspec)
+        mp_tgt0 k_tgt k_src
+        fn tbr ord_cur varg_src varg_tgt
+        (R: A -> Any.t -> Any.t -> iProp)
+        (eqr: Any.t -> Any.t -> Any.t -> Any.t -> Prop)
+
+        (WEAKER: fspec_weaker fsp1 fsp0)
+
+        ctx0 I
+        (ACC: current_iProp ctx0 I)
+
+        (UPDATABLE:
+           I ⊢ #=> (FR ** R a0 mp_src0 mp_tgt0 ** (fsp1.(precond) (Some mn) x varg_src varg_tgt: iProp)))
+
+        (PURE: ord_lt (fsp1.(measure) x) ord_cur /\
+               (tbr = true -> is_pure (fsp1.(measure) x)) /\ (tbr = false -> (fsp1.(measure) x) = ord_top))
+
+        (POST: forall (vret_tgt : Any.t) (mr_src1: Σ) (mp_src1 mp_tgt1 : Any.t) a1
+                      (vret_src: Any.t)
+                      (WLE: le a0 a1)
+                      ctx1
+                      (ACC: current_iProp ctx1 (FR ** R a1 mp_src1 mp_tgt1 ** fsp1.(postcond) (Some mn) x vret_src vret_tgt))
+          ,
+                gpaco8 (_sim_itree (mk_wf R) le) (cpn8 (_sim_itree (mk_wf R) le)) rg rg _ _ eqr true true a
+                       (Any.pair mp_src1 mr_src1↑, k_src (ctx1, vret_src)) (mp_tgt1, k_tgt vret_tgt))
+    :
+      gpaco8 (_sim_itree (mk_wf R) le) (cpn8 (_sim_itree (mk_wf R) le)) r rg _ _ eqr m n a
+             (Any.pair mp_src0 mr_src0, (HoareCall mn tbr ord_cur fsp0 fn varg_src) ctx0 >>= k_src)
+             (mp_tgt0, trigger (Call fn varg_tgt) >>= k_tgt)
+  .
+  Proof.
+    subst. unfold HoareCall, mput, mget, assume, guarantee.
+    ired_both. apply sim_itreeC_spec. econs.
+    hexploit (WEAKER x). i. des.
+    assert (exists mr_src0' rarg_src fr_src0',
+               (<<UPDATABLE: URA.wf (ctx0 ⋅ (mr_src0' ⋅ (rarg_src ⋅ fr_src0')))>>) /\
+               (<<RSRC: R a0 mp_src0 mp_tgt0 mr_src0'>>) /\
+               (<<FRS: FR fr_src0'>>) /\
+               (<<PRE: fsp0.(precond) (Some mn) x_tgt varg_src varg_tgt rarg_src>>)).
+    { inv ACC. uipropall. hexploit UPDATABLE.
+      { eapply URA.wf_mon. eapply GWF. }
+      { eapply IPROP. }
+      { et. }
+      i. des. subst.
+      hexploit PRE; et. i. uipropall. hexploit (H0 b); et.
+      { eapply URA.wf_mon in H. rewrite URA.add_comm in H. eapply URA.wf_mon in H. auto. }
+      { instantiate (1:=a2 ⋅ b0 ⋅ ctx0).
+        replace (b ⋅ (a2 ⋅ b0 ⋅ ctx0)) with (a2 ⋅ b0 ⋅ b ⋅ ctx0); auto. r_solve. }
+      i. des. esplits; et.
+      { replace (ctx0 ⋅ (b0 ⋅ (r1 ⋅ a2))) with (r1 ⋅ (a2 ⋅ b0 ⋅ ctx0)); auto. r_solve. }
+    }
+    des. exists (rarg_src, fr_src0', mr_src0').
+    repeat (ired_both; apply sim_itreeC_spec; econs). unshelve esplits; eauto.
+    { r_wf UPDATABLE0. }
+    repeat (ired_both; apply sim_itreeC_spec; econs). exists x_tgt.
+    repeat (ired_both; apply sim_itreeC_spec; econs). exists varg_tgt.
+    repeat (ired_both; apply sim_itreeC_spec; econs). unshelve esplits; eauto.
+    repeat (ired_both; apply sim_itreeC_spec; econs). unshelve esplits; eauto.
+    { r in MEASURE. des_ifs; ss; des_ifs. eapply Ord.le_lt_lt; et. }
+    { i. spc PURE0. r in MEASURE. des_ifs; ss; des_ifs. }
+    { i. spc PURE1. r in MEASURE. des_ifs; ss; des_ifs. }
+    repeat (ired_both; apply sim_itreeC_spec; econs).
+    { econs; eauto. }
+    i. repeat (ired_both; apply sim_itreeC_spec; econs). i. destruct x0.
+    repeat (ired_both; apply sim_itreeC_spec; econs). inv WF.
+    repeat (ired_both; apply sim_itreeC_spec; econs). i.
+    repeat (ired_both; apply sim_itreeC_spec; econs). i.
+    repeat (ired_both; apply sim_itreeC_spec; econs). i.
+    ired_both. eapply POST; eauto. hexploit POST0. i.
+    uipropall. hexploit (H c); et.
+    { eapply URA.wf_mon. instantiate (1:=fr_src0' ⋅ c0 ⋅ mr_src). r_wf x0. }
+    { instantiate (1:=fr_src0' ⋅ c0 ⋅ mr_src). r_wf x0. }
+    i. des. econs.
+    { instantiate (1:=fr_src0' ⋅ mr_src ⋅ r1). r_wf H0. }
+    esplits; et.
+    eapply RSRC0.
+    eapply URA.wf_mon. instantiate (1:=r1 ⋅ fr_src0' ⋅ c0). r_wf H0.
+  Qed.
+
+  Lemma hcall_clo_ord_weaken
+        Hns Rn Invn
+        (fsp1: fspec)
+        (x: shelve__ fsp1.(meta))
+
+        A (a0: shelve__ A)
+
+        (le: A -> A -> Prop) mn r rg a n m mr_src0 mp_src0
+        (fsp0: fspec)
+        mp_tgt0 k_tgt k_src
+        fn tbr ord_cur varg_src varg_tgt
+        (R: A -> Any.t -> Any.t -> iProp)
+        (eqr: Any.t -> Any.t -> Any.t -> Any.t -> Prop)
+
+        (WEAKER: fspec_weaker fsp1 fsp0)
+
+        ctx0 l
+        (ACC: current_iPropL ctx0 l)
+
+        (UPDATABLE:
+           from_iPropL (fst (alist_pops Hns l)) ⊢ #=> (R a0 mp_src0 mp_tgt0 ** (fsp1.(precond) (Some mn) x varg_src varg_tgt: iProp)))
+
+        (PURE: ord_lt (fsp1.(measure) x) ord_cur /\
+               (tbr = true -> is_pure (fsp1.(measure) x)) /\ (tbr = false -> (fsp1.(measure) x) = ord_top))
+
+        (POST: forall (vret_tgt : Any.t) (mr_src1: Σ) (mp_src1 mp_tgt1 : Any.t) a1
+                      (vret_src: Any.t)
+                      (WLE: le a0 a1)
+                      ctx1
+                      (ACC: current_iPropL ctx1 ((Invn, R a1 mp_src1 mp_tgt1) :: (Rn, fsp1.(postcond) (Some mn) x vret_src vret_tgt) :: snd (alist_pops Hns l)))
+          ,
+            gpaco8 (_sim_itree (mk_wf R) le) (cpn8 (_sim_itree (mk_wf R) le)) rg rg _ _ eqr true true a
+                   (Any.pair mp_src1 mr_src1↑, k_src (ctx1, vret_src)) (mp_tgt1, k_tgt vret_tgt))
+    :
+      gpaco8 (_sim_itree (mk_wf R) le) (cpn8 (_sim_itree (mk_wf R) le)) r rg _ _ eqr m n a
+             (Any.pair mp_src0 mr_src0, (HoareCall mn tbr ord_cur fsp0 fn varg_src) ctx0 >>= k_src)
+             (mp_tgt0, trigger (Call fn varg_tgt) >>= k_tgt)
+  .
+  Proof.
+    subst. eapply hcall_clo_ord_weaken'; et.
+    { instantiate (2:=from_iPropL (snd (alist_pops Hns l))).
+      etrans.
+      { eapply iPropL_alist_pops. }
+      iIntros "[H0 H1]".
+      iPoseProof (UPDATABLE with "H0") as "> [H0 H2]".
+      iModIntro. iFrame.
+    }
+    i. eapply POST; et. red. ss.
+    eapply current_iProp_entail; et.
+    iIntros "[[H0 H1] H2]". iFrame.
+  Qed.
+
+  Lemma hcall_clo_weaken
+        Hns Rn Invn
+        (fsp1: fspec)
+        (x: shelve__ fsp1.(meta))
+
+        A (a0: shelve__ A)
+
+        (le: A -> A -> Prop) mn r rg a n m mr_src0 mp_src0
+        (fsp0: fspec)
+        mp_tgt0 k_tgt k_src
+        fn tbr ord_cur varg_src varg_tgt
+        (R: A -> Any.t -> Any.t -> iProp)
+        (eqr: Any.t -> Any.t -> Any.t -> Any.t -> Prop)
+
+        (WEAKER: fspec_weaker fsp1 fsp0)
+
+        ctx0 l
+        (ACC: current_iPropL ctx0 l)
+
+        (UPDATABLE:
+           from_iPropL (fst (alist_pops Hns l)) ⊢ #=> (R a0 mp_src0 mp_tgt0 ** (fsp1.(precond) (Some mn) x varg_src varg_tgt: iProp)))
+
+        (PURE: ord_lt (fsp1.(measure) x) ord_cur /\
+               (tbr = true -> is_pure (fsp1.(measure) x)) /\ (tbr = false -> (fsp1.(measure) x) = ord_top))
+
+        (POST: forall (vret_tgt : Any.t) (mr_src1: Σ) (mp_src1 mp_tgt1 : Any.t) a1
+                      (vret_src: Any.t)
+                      (WLE: le a0 a1)
+                      ctx1
+                      (ACC: current_iPropL ctx1 (@cons (prod string (bi_car iProp)) (Invn, R a1 mp_src1 mp_tgt1) (@cons (prod string (bi_car iProp)) (Rn, fsp1.(postcond) (Some mn) x vret_src vret_tgt) (snd (alist_pops Hns l)))))
+          ,
+            gpaco8 (_sim_itree (mk_wf R) le) (cpn8 (_sim_itree (mk_wf R) le)) rg rg _ _ eqr true true a
+                   (Any.pair mp_src1 mr_src1↑, k_src (ctx1, vret_src)) (mp_tgt1, k_tgt vret_tgt))
+    :
+      gpaco8 (_sim_itree (mk_wf R) le) (cpn8 (_sim_itree (mk_wf R) le)) r rg _ _ eqr m n a
+             (Any.pair mp_src0 mr_src0, (HoareCall mn tbr ord_cur fsp0 fn varg_src) ctx0 >>= k_src)
+             (mp_tgt0, trigger (Call fn varg_tgt) >>= k_tgt)
+  .
+  Proof.
+    eapply (@hcall_clo_ord_weaken _ _ _); eauto.
+  Qed.
+
+  Lemma hcall_clo
+        Hns Rn Invn
+        X (x: shelve__ X)
+        A (a0: shelve__ A)
+
+        (D: X -> ord)
+        (P: option mname -> X -> Any.t -> Any.t -> Σ -> Prop)
+        (Q: option mname -> X -> Any.t -> Any.t -> Σ -> Prop)
+        (le: A -> A -> Prop) mn r rg a n m mr_src0 mp_src0
+        mp_tgt0 k_tgt k_src
+        fn tbr ord_cur varg_src varg_tgt
+        (R: A -> Any.t -> Any.t -> iProp)
+        (eqr: Any.t -> Any.t -> Any.t -> Any.t -> Prop)
+
+        ctx0 l
+        (ACC: current_iPropL ctx0 l)
+
+        (UPDATABLE:
+           from_iPropL (fst (alist_pops Hns l)) ⊢ #=> (R a0 mp_src0 mp_tgt0 ** (P (Some mn) x varg_src varg_tgt: iProp)))
+
+        (PURE: ord_lt (D x) ord_cur /\
+               (tbr = true -> is_pure (D x)) /\ (tbr = false -> (D x) = ord_top))
+
+        (POST: forall (vret_tgt : Any.t) (mr_src1: Σ) (mp_src1 mp_tgt1 : Any.t) a1
+                      (vret_src: Any.t)
+                      (WLE: le a0 a1)
+                      ctx1
+                      (ACC: current_iPropL ctx1 (@cons (prod string (bi_car iProp)) (Invn, R a1 mp_src1 mp_tgt1) (@cons (prod string (bi_car iProp)) (Rn, Q (Some mn) x vret_src vret_tgt) (snd (alist_pops Hns l)))))
+          ,
+                gpaco8 (_sim_itree (mk_wf R) le) (cpn8 (_sim_itree (mk_wf R) le)) rg rg _ _ eqr true true a
+                       (Any.pair mp_src1 mr_src1↑, k_src (ctx1, vret_src)) (mp_tgt1, k_tgt vret_tgt))
+    :
+      gpaco8 (_sim_itree (mk_wf R) le) (cpn8 (_sim_itree (mk_wf R) le)) r rg _ _ eqr m n a
+             (Any.pair mp_src0 mr_src0, (HoareCall mn tbr ord_cur (mk_fspec D P Q) fn varg_src) ctx0 >>= k_src)
+             (mp_tgt0, trigger (Call fn varg_tgt) >>= k_tgt)
+  .
+  Proof.
+    eapply hcall_clo_weaken; eauto.
+    { refl. }
+    { eauto. }
+    { eauto. }
+    { eauto. }
+  Qed.
+
+  Lemma harg_clo
+        A Rn Invn
+        mn r rg
+        X (P: option mname -> X -> Any.t -> Any.t -> Σ -> Prop) varg
+        mpr_src mp_tgt f_tgt k_src
+        a (le: A -> A -> Prop)
+        (R: A -> Any.t -> Any.t -> iProp)
+        (eqr: Any.t -> Any.t -> Any.t -> Any.t -> Prop)
+        (WF: mk_wf R a (mpr_src, mp_tgt))
+        m n
+        (ARG:
+           forall x varg_src
+                  ctx (mr_src: Σ) mp_src
+                  (ACC: current_iPropL ctx (@cons (prod string (bi_car iProp)) (Rn, P mn x varg_src varg) (@cons (prod string (bi_car iProp)) (Invn, R a mp_src mp_tgt) (@nil (prod string (bi_car iProp)))))),
+             gpaco8 (_sim_itree (mk_wf R) le) (cpn8 (_sim_itree (mk_wf R) le)) r rg _ _ eqr true n a
+                    (Any.pair mp_src mr_src↑, k_src (ctx, ((mn, x), varg_src)))
+                    (mp_tgt, f_tgt))
+    :
+      gpaco8 (_sim_itree (mk_wf R) le) (cpn8 (_sim_itree (mk_wf R) le)) r rg _ _ eqr m n a
+             (mpr_src, (HoareFunArg P (mn, varg) >>= k_src))
+             (mp_tgt, f_tgt)
+  .
+  Proof.
+    inv WF.
+    unfold HoareFunArg, mput, mget, assume, guarantee.
+    repeat (ired_both; apply sim_itreeC_spec; econs). intro x.
+    repeat (ired_both; apply sim_itreeC_spec; econs). intro varg_src.
+    repeat (ired_both; apply sim_itreeC_spec; econs). intros (rarg_src, ctx).
+    repeat (ired_both; apply sim_itreeC_spec; econs). intros VALID.
+    repeat (ired_both; apply sim_itreeC_spec; econs). intro PRE.
+    ired_both. eapply ARG; et.
+    red. econs.
+    { instantiate (1:=rarg_src ⋅ mr_src). r_wf VALID. }
+    { ss. red. uipropall. esplits; et.
+      { rewrite URA.unit_id. et. }
+      { eapply RSRC; et. eapply URA.wf_mon. instantiate (1:=(ctx ⋅ rarg_src)). r_wf VALID. }
+      { red. uipropall. }
+    }
+  Qed.
+
+  Lemma hret_clo
+        A (a: shelve__ A)
+        mn r rg n m mr_src mp_src a0
+        X (Q: option mname -> X -> Any.t -> Any.t -> Σ -> Prop)
+        x vret_src vret_tgt
+        mp_tgt
+        (le: A -> A -> Prop)
+        (eqr: Any.t -> Any.t -> Any.t -> Any.t -> Prop)
+        (R: A -> Any.t -> Any.t -> iProp)
+
+        ctx l
+        (ACC: current_iPropL ctx l)
+
+        (WLE: le a0 a)
+
+        (UPDATABLE:
+           (from_iPropL l) ⊢ #=> (R a mp_src mp_tgt ** (Q mn x vret_src vret_tgt: iProp)))
+
+        (EQ: forall (mr_src1: Σ) (WLE: le a0 a) (WF: mk_wf R a (Any.pair mp_src mr_src1↑, mp_tgt)),
+            eqr (Any.pair mp_src mr_src1↑) mp_tgt vret_tgt vret_tgt)
+    :
+      gpaco8 (_sim_itree (mk_wf R) le) (cpn8 (_sim_itree (mk_wf R) le)) r rg _ _ eqr m n a0
+             (Any.pair mp_src mr_src, (HoareFunRet Q mn x (ctx, vret_src)))
+             (mp_tgt, (Ret vret_tgt))
+  .
+  Proof.
+    subst. unfold HoareFunRet, mput, mget, guarantee.
+    repeat (ired_both; apply sim_itreeC_spec; econs). exists vret_tgt.
+    repeat (ired_both; apply sim_itreeC_spec; econs).
+    assert (exists mr_src1 rret_src,
+               (<<UPDATABLE: URA.wf (ctx ⋅ (mr_src1 ⋅ rret_src))>>) /\
+               (<<RSRC: R a mp_src mp_tgt mr_src1>>) /\
+               (<<PRE: Q mn x vret_src vret_tgt rret_src>>)).
+    { red in ACC. inv ACC. uipropall.
+      hexploit (UPDATABLE r0); et.
+      { eapply URA.wf_mon; et. }
+      i. des. subst. exists a1, b. splits; et.
+      replace (ctx ⋅ (a1 ⋅ b)) with (a1 ⋅ b ⋅ ctx); et.
+      r_solve.
+    }
+    des. exists (rret_src, mr_src1).
+    repeat (ired_both; apply sim_itreeC_spec; econs).
+    repeat (ired_both; apply sim_itreeC_spec; econs). unshelve esplits.
+    { r_wf UPDATABLE0. }
+    repeat (ired_both; apply sim_itreeC_spec; econs). unshelve esplits; eauto.
+    repeat (ired_both; apply sim_itreeC_spec; econs).
+    eapply EQ; et. econs; et.
+  Qed.
+
+  Lemma APC_start_clo
+        (at_most: Ord.t)
+        (o: ord)
+        A mn r rg a m n mp_src0
+        k_src
+        (wf: A -> Any.t * Any.t -> Prop)
+        (le: A -> A -> Prop)
+        (eqr: Any.t -> Any.t -> Any.t -> Any.t -> Prop)
+        stb itr_tgt ctx
+
+        (POST: gpaco8 (_sim_itree wf le) (cpn8 (_sim_itree wf le)) r rg _ _ eqr true n a
+                      (mp_src0,
+                       (interp_hCallE_tgt mn stb o (_APC at_most) ctx)>>= k_src)
+                      (itr_tgt))
+    :
+      gpaco8 (_sim_itree wf le) (cpn8 (_sim_itree wf le)) r rg _ _ eqr m n a
+             (mp_src0,
+              (interp_hCallE_tgt mn stb o APC ctx) >>= k_src)
+             (itr_tgt).
+  Proof.
+    subst. unfold APC. destruct itr_tgt.
+    ired_both. apply sim_itreeC_spec. eapply sim_itreeC_choose_src.
+    exists at_most.
+    repeat (ired_both; apply sim_itreeC_spec; econs).
+    ired_both. et.
+    Unshelve. all: ss.
+  Qed.
+
+  Lemma APC_stop_clo
+        (o: ord)
+        A mn r rg a n m mp_src0
+        k_src
+        (at_most: Ord.t)
+        (wf: A -> Any.t * Any.t -> Prop)
+        (le: A -> A -> Prop)
+        (eqr: Any.t -> Any.t -> Any.t -> Any.t -> Prop)
+        stb itr_tgt ctx
+
+        (POST: gpaco8 (_sim_itree wf le) (cpn8 (_sim_itree wf le)) r rg _ _ eqr true n a
+                      (mp_src0, k_src (ctx, ()))
+                      (itr_tgt))
+    :
+      gpaco8 (_sim_itree wf le) (cpn8 (_sim_itree wf le)) r rg _ _ eqr m n a
+              (mp_src0,
+              (interp_hCallE_tgt mn stb o (_APC at_most) ctx) >>= k_src)
+             (itr_tgt).
+  Proof.
+    subst. destruct itr_tgt.
+    rewrite unfold_APC. ired_l. apply sim_itreeC_spec. eapply sim_itreeC_choose_src.
+    exists true. ired_l. apply sim_itreeC_spec. eapply sim_itreeC_tau_src.
+    ired_both. et.
+  Qed.
+
+  Lemma APC_step_clo
+        (fn: gname) (args: Any.t) (next: Ord.t)
+
+        (o: ord)
+        A mn r rg a n m mp_src0
+        k_src ctx0
+        (at_most: Ord.t)
+        (wf: A -> Any.t * Any.t -> Prop)
+        (le: A -> A -> Prop)
+        (eqr: Any.t -> Any.t -> Any.t -> Any.t -> Prop)
+        stb itr_tgt
+
+        (fsp: fspec)
+        (FIND: stb fn = Some fsp)
+        (NEXT: (next < at_most)%ord)
+
+        (POST: gpaco8 (_sim_itree wf le) (cpn8 (_sim_itree wf le)) r rg _ _ eqr true n a
+                      (mp_src0,
+                       ('(ctx1, _) <- (HoareCall mn true o fsp fn args ctx0);;
+                        Tau (ITree.bind (interp_hCallE_tgt mn stb o (_APC next) ctx1) k_src)))
+                      (itr_tgt))
+    :
+      gpaco8 (_sim_itree wf le) (cpn8 (_sim_itree wf le)) r rg _ _ eqr m n a
+             (mp_src0, (interp_hCallE_tgt mn stb o (_APC at_most) ctx0) >>= k_src)
+             (itr_tgt).
+  Proof.
+    subst. destruct itr_tgt.
+    rewrite unfold_APC. ired_l. apply sim_itreeC_spec. eapply sim_itreeC_choose_src.
+    exists false. ired_l. apply sim_itreeC_spec. eapply sim_itreeC_tau_src.
+    ired_l. apply sim_itreeC_spec. eapply sim_itreeC_choose_src.
+    exists next. ired_l. apply sim_itreeC_spec. eapply sim_itreeC_tau_src.
+    ired_l. unfold guarantee. ired_l. apply sim_itreeC_spec. eapply sim_itreeC_choose_src.
+    split.
+    { auto. }
+    ired_l. apply sim_itreeC_spec. eapply sim_itreeC_tau_src.
+    ired_l. apply sim_itreeC_spec. eapply sim_itreeC_choose_src.
+    exists (fn, args).
+    ired_l. apply sim_itreeC_spec. eapply sim_itreeC_tau_src.
+    ired_l. ss. rewrite FIND. ss. subst. ired_l.
+    ss. ired_l.
+    match goal with
+    | [SIM: gpaco8 _ _ _ _ _ _ _ _ _ _ ?i0 _ |- gpaco8 _ _ _ _ _ _ _ _ _ _ ?i1 _] =>
+      replace i1 with i0; et
+    end.
+    f_equal. grind.
+  Qed.
+
+  Lemma trivial_init_clo
+        A wf (le: A -> A -> Prop) r rg w arg mrp_src mp_tgt itr_tgt mn stb body RR
+        m n
+        (INIT:
+           gpaco8 (_sim_itree wf le) (cpn8 (_sim_itree wf le)) r rg Any.t Any.t
+                  RR true n w
+                  (mrp_src, fun_to_tgt mn stb (mk_specbody fspec_trivial body) arg)
+                  (mp_tgt, itr_tgt))
+    :
+      gpaco8 (_sim_itree wf le) (cpn8 (_sim_itree wf le)) r rg Any.t Any.t
+             RR m n w
+             (mrp_src, KModSem.disclose_ksb_tgt mn stb (ksb_trivial body) arg)
+             (mp_tgt, itr_tgt).
+  Proof.
+    unfold KModSem.disclose_ksb_tgt.
+    apply sim_itreeC_spec. econs; eauto. i. destruct x; et.
+  Qed.
+
+End HLEMMAS.
+
+
+Ltac prep := ired_both.
+
+Ltac _force_l :=
+  prep;
+  match goal with
+  | [ |- (gpaco8 (_sim_itree _ _) _ _ _ _ _ _ _ _ _ (_, unwrapN ?ox >>= _) (_, _)) ] =>
+    let tvar := fresh "tmp" in
+    let thyp := fresh "TMP" in
+    remember (unwrapN ox) as tvar eqn:thyp; unfold unwrapN in thyp; subst tvar;
+    let name := fresh "_UNWRAPN" in
+    destruct (ox) eqn:name; [|exfalso]; cycle 1
+  | [ |- (gpaco8 (_sim_itree _ _) _ _ _ _ _ _ _ _ _ (_, guarantee ?P >>= _) (_, _)) ] =>
+    let tvar := fresh "tmp" in
+    let thyp := fresh "TMP" in
+    remember (guarantee P) as tvar eqn:thyp; unfold guarantee in thyp; subst tvar;
+    let name := fresh "_GUARANTEE" in
+    destruct (classic P) as [name|name]; [ired_both; apply sim_itreeC_spec; eapply sim_itreeC_choose_src; [exists name]|contradict name]; cycle 1
+
+  | [ |- (gpaco8 (_sim_itree _ _) _ _ _ _ _ _ _ _ _ (_, ITree.bind' _ (interp _ guarantee ?P) (_, _))) ] =>
+    let tvar := fresh "tmp" in
+    let thyp := fresh "TMP" in
+    remember (guarantee P) as tvar eqn:thyp; unfold guarantee in thyp; subst tvar;
+    let name := fresh "_GUARANTEE" in
+    destruct (classic P) as [name|name]; [ired_both; apply sim_itreeC_spec; eapply sim_itreeC_choose_src; [exists name]|contradict name]; cycle 1
+
+   (* TODO: handle interp_hCallE_tgt better and remove this case *)
+  | [ |- (gpaco8 (_sim_itree _ _) _ _ _ _ _ _ _ _ _ (_, ITree.bind' _ (interp _ (guarantee ?P ))) (_, _)) ] =>
+    let tvar := fresh "tmp" in
+    let thyp := fresh "TMP" in
+    remember (guarantee P) as tvar eqn:thyp; unfold guarantee in thyp; subst tvar;
+    let name := fresh "_GUARANTEE" in
+    destruct (classic P) as [name|name]; [ired_both; apply sim_itreeC_spec; eapply sim_itreeC_choose_src; [exists name]|contradict name]; cycle 1; clear name
+
+  | [ |- (gpaco8 (_sim_itree _ _) _ _ _ _ _ _ _ _ _ (_, ?i_src) (_, ?i_tgt)) ] =>
+    seal i_tgt; apply sim_itreeC_spec; econs; unseal i_tgt
+  end
+.
+
+Ltac _force_r :=
+  prep;
+  match goal with
+  | [ |- (gpaco8 (_sim_itree _ _) _ _ _ _ _ _ _ _ _ (_, _) (_, unwrapU ?ox >>= _)) ] =>
+    let tvar := fresh "tmp" in
+    let thyp := fresh "TMP" in
+    remember (unwrapU ox) as tvar eqn:thyp; unfold unwrapU in thyp; subst tvar;
+    let name := fresh "_UNWRAPU" in
+    destruct (ox) eqn:name; [|exfalso]; cycle 1
+  | [ |- (gpaco8 (_sim_itree _ _) _ _ _ _ _ _ _ _ _ (_, _) (_, assume ?P >>= _)) ] =>
+    let tvar := fresh "tmp" in
+    let thyp := fresh "TMP" in
+    remember (assume P) as tvar eqn:thyp; unfold assume in thyp; subst tvar;
+    let name := fresh "_ASSUME" in
+    destruct (classic P) as [name|name]; [ired_both; apply sim_itreeC_spec; eapply sim_itreeC_take_tgt; [exists name]|contradict name]; cycle 1
+
+  | [ |- (gpaco8 (_sim_itree _ _) _ _ _ _ _ _ _ _ _ (_, ?i_src) (_, ?i_tgt)) ] =>
+    seal i_src; apply sim_itreeC_spec; econs; unseal i_src
+  end
+.
+
+Ltac _step :=
+  match goal with
+  (*** blacklisting ***)
+  (* | [ |- (gpaco5 (_sim_itree wf) _ _ _ _ (_, trigger (Choose _) >>= _) (_, ?i_tgt)) ] => idtac *)
+  | [ |- (gpaco8 (_sim_itree _ _) _ _ _ _ _ _ _ _ _ (_, triggerUB >>= _) (_, _)) ] =>
+    unfold triggerUB; ired_l; _step; done
+  | [ |- (gpaco8 (_sim_itree _ _) _ _ _ _ _ _ _ _ _ (_, unwrapU ?ox >>= _) (_, _)) ] =>
+    let tvar := fresh "tmp" in
+    let thyp := fresh "TMP" in
+    remember (unwrapU ox) as tvar eqn:thyp; unfold unwrapU in thyp; subst tvar;
+    let name := fresh "_UNWRAPU" in
+    destruct (ox) eqn:name; [|unfold triggerUB; ired_both; _force_l; ss; fail]
+  | [ |- (gpaco8 (_sim_itree _ _) _ _ _ _ _ _ _ _ _ (_, assume ?P >>= _) (_, _)) ] =>
+    let tvar := fresh "tmp" in
+    let thyp := fresh "TMP" in
+    remember (assume P) as tvar eqn:thyp; unfold assume in thyp; subst tvar;
+    let name := fresh "_ASSUME" in
+    ired_both; apply sim_itreeC_spec; eapply sim_itreeC_take_src; intro name
+
+  (*** blacklisting ***)
+  (* | [ |- (gpaco5 (_sim_itree wf) _ _ _ _ (_, _) (_, trigger (Take _) >>= _)) ] => idtac *)
+  | [ |- (gpaco8 (_sim_itree _ _) _ _ _ _ _ _ _ _ _ (_, triggerNB >>= _) (_, _)) ] =>
+    unfold triggerNB; ired_r; _step; done
+  | [ |- (gpaco8 (_sim_itree _ _) _ _ _ _ _ _ _ _ _ (_, _) (_, unwrapN ?ox >>= _)) ] =>
+    let tvar := fresh "tmp" in
+    let thyp := fresh "TMP" in
+    remember (unwrapN ox) as tvar eqn:thyp; unfold unwrapN in thyp; subst tvar;
+    let name := fresh "_UNWRAPN" in
+    destruct (ox) eqn:name; [|unfold triggerNB; ired_both; _force_r; ss; fail]
+  | [ |- (gpaco8 (_sim_itree _ _) _ _ _ _ _ _ _ _ _ (_, _) (_, guarantee ?P >>= _)) ] =>
+    let tvar := fresh "tmp" in
+    let thyp := fresh "TMP" in
+    remember (guarantee P) as tvar eqn:thyp; unfold guarantee in thyp; subst tvar;
+    let name := fresh "_GUARANTEE" in
+    ired_both; apply sim_itreeC_spec; eapply sim_itreeC_choose_tgt; intro name
+
+
+
+  | _ => (*** default ***)
+    eapply safe_sim_sim; econs; i
+  end;
+  match goal with
+  | [ |- exists (_: unit), _ ] => esplits; [eauto|..]; i
+  | [ |- exists _, _ ] => fail 1
+  | _ => idtac
+  end
+.
+Ltac _steps := repeat ((*** pre processing ***) prep; try _step; (*** post processing ***) simpl).
+
+Ltac steps := repeat ((*** pre processing ***) prep; try _step; (*** post processing ***) simpl; des_ifs_safe).
+Ltac force_l := _force_l.
+Ltac force_r := _force_r.
+
+Notation "wf n '------------------------------------------------------------------' src0 tgt0 '------------------------------------------------------------------' src1 '------------------------------------------------------------------' src2 tgt2"
+  :=
+    (gpaco8 (_sim_itree wf _) _ _ _ _ _ _ _ _ n ((Any.pair src0 src1), src2) (tgt0, tgt2))
+      (at level 60,
+       format "wf  n '//' '------------------------------------------------------------------' '//' src0 '//' tgt0 '//' '------------------------------------------------------------------' '//' src1 '//' '------------------------------------------------------------------' '//' src2 '//' '//' '//' tgt2 '//' ").
+
+Notation "wf n '------------------------------------------------------------------' src0 tgt0 '------------------------------------------------------------------' '------------------------------------------------------------------' src2 tgt2"
+  :=
+    (gpaco8 (_sim_itree wf _) _ _ _ _ _ _ _ _ n (src0, src2) (tgt0, tgt2))
+      (at level 60,
+       format "wf  n '//' '------------------------------------------------------------------' '//' src0 '//' tgt0 '//' '------------------------------------------------------------------' '//' '//' '------------------------------------------------------------------' '//' src2 '//' '//' '//' tgt2 '//' ").
+
+Section TEST.
+  Context `{Σ: GRA.t}.
+  Let wf := (mk_wf (fun (_ : unit) (_ _ : Any.t) => bi_pure True)).
+  Let le := fun (_ _: unit) => True.
+  Variable (srcs0 tgts0: Any.t).
+
+  Goal gpaco8 (_sim_itree wf le) (cpn8 (_sim_itree wf le)) bot8 bot8 Any.t Any.t (fun _ _ => eq) false false tt
+       (srcs0, triggerUB >>= idK) (tgts0, triggerUB >>= idK).
+  Proof.
+    steps.
+  Qed.
+
+  Goal gpaco8 (_sim_itree wf le) (cpn8 (_sim_itree wf le)) bot8 bot8 Any.t Any.t (fun _ _ => eq) false false tt
+       (srcs0, triggerNB >>= idK) (tgts0, triggerNB >>= idK).
+  Proof.
+    steps.
+  Qed.
+
+End TEST.
+
+
+Ltac astep_full _fn _args _next _n1 :=
+  eapply (@APC_step_clo _ _fn _args _next _n1);
+  [(try by ((try stb_tac); refl))|
+   oauto|
+  ].
+
+Ltac astep _fn _args :=
+  eapply (@APC_step_clo _ _fn _args);
+  [(try by ((try stb_tac); refl))|
+   oauto|
+  ].
+
+Ltac acatch :=
+  match goal with
+  | [ |- (gpaco8 (_sim_itree _ _) _ _ _ _ _ _ _ _ _ (_, _) (_, trigger (Call ?fn ?args) >>= _)) ] =>
+    astep fn args
+  end.
+
+Ltac astart _at_most :=
+  eapply (@APC_start_clo _ _at_most)
+.
+
+Ltac astop :=
+  match goal with
+  | [ |- (gpaco8 (_sim_itree _ _) _ _ _ _ _ _ _ _ _ (_, interp_hCallE_tgt _ _ _ APC _ >>= _) (_, _)) ] => astart 0
+  | _ => idtac
+  end;
+  eapply APC_stop_clo.
+
+Ltac init :=
+  let varg_src := fresh "varg_src" in
+  let mn := fresh "mn" in
+  let varg := fresh "varg" in
+  let EQ := fresh "EQ" in
+  let w := fresh "w" in
+  let mrp_src := fresh "mrp_src" in
+  let mp_tgt := fresh "mp_tgt" in
+  let WF := fresh "WF" in
+  split; ss; intros varg_src [mn varg] EQ w mrp_src mp_tgt WF;
+  try subst varg_src; cbn; ginit;
+  match goal with
+  | |- gpaco8 _ _ _ _ _ _ _ _ _ _ (_, KModSem.disclose_ksb_tgt _ _ (ksb_trivial _) _) _ =>
+    eapply trivial_init_clo;
+    try (unfold fun_to_tgt, cfunN, cfunU, KModSem.disclose_ksb_tgt, fun_to_tgt);
+    rewrite HoareFun_parse; simpl
+  | |- gpaco8 _ _ _ _ _ _ _ _ _ _ (_, KModSem.disclose_ksb_tgt _ _ _ _) _ =>
+    try (unfold fun_to_tgt, cfunN, cfunU, KModSem.disclose_ksb_tgt, fun_to_tgt);
+    simpl;
+    apply sim_itreeC_spec; apply sim_itreeC_take_src; intros [];rewrite HoareFun_parse; simpl
+  | |- _ =>
+    try (unfold fun_to_tgt, cfunN, cfunU; rewrite HoareFun_parse); simpl
+  end.
+
+Ltac harg :=
+  let PRE := constr:("PRE") in
+  let INV := constr:("INV") in
+  eapply (@harg_clo _ _ PRE INV);
+  [eassumption
+  |
+  ]; i.
+
+Tactic Notation "hret" uconstr(a) :=
+  eapply (@hret_clo _ _ a); unshelve_goal;
+  [eassumption
+  |
+  |start_ipm_proof
+  |try by (i; (try unfold lift_rel); esplits; et)
+  ].
+
+Tactic Notation "hcall" uconstr(x) uconstr(a) "with" constr(Hns) :=
+  let POST := get_fresh_name_tac "POST" in
+  let INV := get_fresh_name_tac "INV" in
+  let Hns := select_ihyps Hns in
+  eapply (@hcall_clo _ Hns POST INV _ x _ a);
+  unshelve_goal;
+  [eassumption
+  |start_ipm_proof
+  |
+  |on_current ltac:(fun H => try clear H); i; on_current ltac:(fun H => simpl in H)
+  ].
+
+Tactic Notation "hcall_weaken" uconstr(fsp) uconstr(x) uconstr(a) "with" constr(Hns) :=
+  let POST := get_fresh_name_tac "POST" in
+  let INV := get_fresh_name_tac "INV" in
+  let Hns := select_ihyps Hns in
+  eapply (@hcall_clo_weaken _ Hns POST INV fsp x _ a);
+  unshelve_goal;
+  [
+  |eassumption
+  |start_ipm_proof
+  |
+  |on_current ltac:(fun H => try clear H); i; on_current ltac:(fun H => simpl in H)
+  ].
+
+Ltac iarg :=
+  let PRE := constr:("PRE") in
+  let INV := constr:("INV") in
+  let CLOSED := constr:("☃CLOSED") in
+  eapply (@harg_clo _ _ PRE INV);
+  [eassumption
+  |
+  ];
+  i;
+  mDesSep PRE as CLOSED PRE;
+  match goal with
+  | [ |- (gpaco8 _ _ _ _ _ _ _ _ _ ?w _ _)] =>
+    destruct w as [?|[?mp_src ?mp_tgt]]; simpl;
+    [
+        |mAssertPure False; ss; iDestruct "INV" as "[INV _]"; iApply (inv_closed_unique with "☃CLOSED INV")
+    ]
+  end.
+
+Tactic Notation "icall_open" uconstr(x) "with" constr(Hns) :=
+  let POST := get_fresh_name_tac "POST" in
+  let INV := constr:("☃CLOSED") in
+  let Hns := select_ihyps Hns in
+  let Hns := constr:("☃CLOSED"::Hns) in
+  eapply (@hcall_clo _ Hns POST INV _ x _ (inr (_, _)));
+  unshelve_goal;
+  [eassumption
+  |start_ipm_proof; iSplitL "☃CLOSED"; [iModIntro; iSplitL "☃CLOSED"; [iExact "☃CLOSED"|ss]|]
+  |
+  |
+  on_current ltac:(fun H => try clear H);
+  intros ? ? ? ? [|[?mp_src ?mp_tgt]]; i; simpl;
+  on_current ltac:(fun H => simpl in H);
+  [exfalso; match goal with | H: inv_le _ _ _ |- _ => cbn in H; inv H end
+  |mDesSep "☃CLOSED" as "☃CLOSED" "☃TMP"; mPure "☃TMP" as [[] []]
+  ]
+  ].
+
+Tactic Notation "icall_weaken" uconstr(ftsp) uconstr(x) uconstr(a) "with" constr(Hns) :=
+  let POST := get_fresh_name_tac "POST" in
+  let INV := get_fresh_name_tac "INV" in
+  let CLOSED := constr:("☃CLOSED") in
+  let TMP := constr:("☃TMP") in
+  let Hns := select_ihyps Hns in
+  let Hns := constr:("☃CLOSED"::Hns) in
+  eapply (@hcall_clo_weaken _ Hns POST INV ftsp x _ (inl a));
+  unshelve_goal;
+  [|eassumption
+   |start_ipm_proof; iFrame "☃CLOSED"
+   |
+   |on_current ltac:(fun H => try clear H);
+    intros ? ? ? ? [|[?mp_src ?mp_tgt]]; i; simpl;
+    on_current ltac:(fun H => simpl in H);
+    [
+      mDesSep POST as "☃CLOSED" POST
+    |
+    mDesSep INV as "☃CLOSED" INV;
+    mDesSep POST as "☃TMP" POST;
+    mAssertPure False; [iApply (inv_closed_unique with "☃TMP ☃CLOSED")|ss]
+    ]
+  ].
+
+Tactic Notation "iret" uconstr(a) :=
+  eapply (@hret_clo _ _ (inl a)); unshelve_goal;
+  [eassumption
+  |
+  |start_ipm_proof; iFrame "☃CLOSED"
+  |try by (i; (try unfold lift_rel); esplits; et)
+  ].
+
+
+Global Opaque _APC APC interp interp_hCallE_tgt.
+
+Global Opaque HoareFun HoareFunArg HoareFunRet HoareCall.
+
+Definition __hide_mark A (a : A) : A := a.
+Lemma intro_hide_mark: forall A (a: A), a = __hide_mark a. refl. Qed.
+
+Ltac hide_k :=
+  match goal with
+  | [ |- (gpaco8 _ _ _ _ _ _ _ _ _ _ (_, ?isrc >>= ?ksrc) (_, ?itgt >>= ?ktgt)) ] =>
+    erewrite intro_hide_mark with (a:=ksrc);
+    erewrite intro_hide_mark with (a:=ktgt);
+    let name0 := fresh "__KSRC__" in set (__hide_mark ksrc) as name0; move name0 at top;
+    let name0 := fresh "__KTGT__" in set (__hide_mark ktgt) as name0; move name0 at top
+  end.
+
+Ltac unhide_k :=
+  do 2 match goal with
+  | [ H := __hide_mark _ |- _ ] => subst H
+  end;
+  rewrite <- ! intro_hide_mark
+.
+
+Ltac deflag :=
+  match goal with
+  | [ |- (gpaco8 _ _ _ _ _ _ _ true true _ _ _) ] =>
+    eapply sim_itree_progress_flag
+  | [ |- (gpaco8 _ _ _ _ _ _ _ _ _ _ _ _) ] =>
+    eapply sim_itree_flag_down
+  | _ => fail
+  end.
